mmu_configuration proved

L3_Lib/L3_Hoare_Logic.thy
@@ -5,14 +5,16 @@ begin
 
 
 
-definition l3_valid where 
+definition 
+  l3_valid ::  "('s \<Rightarrow> bool) \<Rightarrow> ('s \<Rightarrow> 'r \<times> 's) \<Rightarrow> ('r \<Rightarrow> 's \<Rightarrow> bool) \<Rightarrow> bool"
+where 
   "l3_valid P f P' \<equiv> \<forall>s s' r. f s = (r, s') \<longrightarrow> P s \<longrightarrow> P' r s'"
 
 
 named_theorems wp_pre
 
 lemma l3_valid_weak_pre[wp_pre]:
-  "\<lbrakk> l3_valid P f Q'; (\<And>s. P' s \<Longrightarrow> P s) \<rbrakk> \<Longrightarrow> l3_valid P' f Q'"
+  "\<lbrakk> l3_valid P f Q; (\<And>s. P' s \<Longrightarrow> P s) \<rbrakk> \<Longrightarrow> l3_valid P' f Q"
   by (simp add: l3_valid_def)
 
 named_theorems wp
@@ -32,7 +34,7 @@ lemma l3_valid_bind:
   by (clarsimp simp: l3_valid_def)
 
 lemma l3_valid_bind_weak[wp]:
-  "\<lbrakk> \<And>r. l3_valid (P1 r) (g r) P2; l3_valid P f P1 \<rbrakk> \<Longrightarrow> l3_valid P (bind f g) P2"
+  "\<lbrakk> \<And>r. l3_valid (P' r) (g r) Q; l3_valid P f P' \<rbrakk> \<Longrightarrow> l3_valid P (bind f g) Q"
   by (simp add: l3_valid_def bind_def split: prod.splits)
 
 
@@ -44,15 +46,14 @@ lemma update_state_weak[wp]:
   "l3_valid (\<lambda>s. \<forall>r. P r (f s)) (update_state f) P"
   by (clarsimp simp: l3_valid_def update_state_def)
 
-lemma extend_state_weak:
+lemma extend_state_weak [wp]:
   "l3_valid (\<lambda>s. P (fst (f (v, s))) (snd (snd (f (v, s))))) (extend_state v f) P"
   by (clarsimp simp: l3_valid_def extend_state_def split_def Let_def)
 
 
-lemma trim_state_weak:
+lemma trim_state_weak [wp]:
   "l3_valid (\<lambda>s. \<forall>a b. P (fst (f b)) (a, snd (f b)) ) (trim_state f ) P"
   by (clarsimp simp: l3_valid_def trim_state_def split_def Let_def)
-
 
 
 end
