TLB_Page_Tables/MMU_Translate_Concrete.thy
@@ -2,127 +2,147 @@ theory MMU_Translate_Concrete
 imports  L3_LIB.L3_Hoare_Logic
          MMU_Translate_Refine
          MMU_ARM.ARM_Monadic
+        MMU_Configuration
 begin
 
+(* write the real lemma, first in terms of l3 *)
+
+term l3_valid
+
+lemma  conj_post:
+ "\<lbrakk>l3_valid P' f Q'; l3_valid P' f Q'' \<rbrakk> \<Longrightarrow> l3_valid P' f (\<lambda>r s. Q' r s \<and> Q'' r s)"
+  by (simp add: l3_valid_def)
+
+term
+  "corres sr r P P' f f'"
+
+lemma
+  "corres (\<lambda>s t. MMU_config_assert_isa s \<and> tlb_rel s (typ_tlb t) \<and> dtlb_consistent (typ_tlb t) (Addr va) \<and> unitlb_consistent (typ_tlb t) (Addr va))
+          (\<lambda>(pa', mematr) adrdesc. pa' = Addr (paddress (adrdesc)) \<and> 
+             mematr = mematr_typcast (AddressDescriptor.memattrs (adrdesc)))
+          (\<lambda>_. True) (\<lambda>_. True) 
+          (mmu_translate  (Addr va) siz ispriv iswrite True) 
+          (TranslateAddress (va , ispriv, iswrite, siz, True))"
+  apply (unfold  TranslateAddress_def)
+  apply (simp flip: bind_assoc)
 
 
-declare return_def [simp add]
+oops
+
+(*declare for_loop.simps [simp add]*)
+
+lemma abc:
+  "l3_valid (\<lambda>s. P () (snd (mainTLB_evict () s)) ) (mainTLB_evict ()) P"
+  apply (clarsimp simp: mainTLB_evict_def)
+    apply ((rule wp)+ ; (clarsimp simp: write'unified_mainTLB_def mainTLBEntries_def)?)
+    apply ((rule wp)+ ; (clarsimp simp:)?)
+
+sorry
+
+lemma abc':
+  "l3_valid (\<lambda>s. P () (snd (microDataTLB_evict () s)) ) (microDataTLB_evict ()) P"
+  apply (clarsimp simp: microDataTLB_evict_def)
+  apply ((rule wp)+ ; (clarsimp simp: write'DataTLB_def microDataTLBEntries_def)?)
+    apply ((rule wp)+ ; (clarsimp simp:)?)
+   apply (clarsimp simp: for_loop.simps)
+ 
+sorry
+
+lemma abc'':
+  "l3_valid (\<lambda>s. P () (snd (microInstrTLB_evict () s)) ) (microInstrTLB_evict ()) P"
+
+sorry
+
+lemma 
+  "l3_valid (\<lambda>s. MMU_config_assert_isa s \<and> tlb_rel s (typ_tlb t) \<and> dtlb_consistent (typ_tlb t) (Addr va) \<and> unitlb_consistent (typ_tlb t) (Addr va))
+      (TranslateAddress (va , ispriv, iswrite, siz, True))
+        (\<lambda>adrdesc s'. 
+           MMU_config_assert_isa s' \<and> 
+           (mmu_translate  (Addr va) siz ispriv iswrite True (t :: 'a tlb_state_scheme) = ((pa', mematr), t') \<longrightarrow>
+           pa' = Addr (paddress (adrdesc)) \<and> 
+           mematr = mematr_typcast (AddressDescriptor.memattrs (adrdesc)) \<and> tlb_rel s' (typ_tlb t') \<and>
+           dtlb_consistent (typ_tlb t') (Addr va) \<and> unitlb_consistent (typ_tlb t') (Addr va)))"
+  apply (rule conj_post)
+   apply (rule_tac P = "MMU_config_assert_isa"  in  wp_pre)
+    prefer 2
+    apply clarsimp
+   apply (clarsimp simp: l3_valid_def)
+   apply (insert mmu_config_TranslateAddress [of va ispriv iswrite siz]) [1]
+   apply (clarsimp simp: mmu_config_def)
+   apply force
+  apply (clarsimp simp: TranslateAddress_def)
+  apply (rule l3_valid_bind_weak)
+  apply ((rule wp)+ ; clarsimp?)
+   apply (rule abc)
+    apply clarsimp
+ apply (rule abc')
+    apply clarsimp
+apply (rule abc'')
+    apply clarsimp
+oops
+term mainTLB_evict
+declare [[show_types]]
+
+lemma
+  "l3_valid (\<lambda>s. Q' () (s \<lparr>main_TLB := main_TLB s \<rparr>)  ) (mainTLB_evict ()) Q'"
+
+oops
 
 
-definition 
-  MMU_config_assert_isa :: "'a state_scheme \<Rightarrow> bool"
-where
-  "MMU_config_assert_isa s \<equiv>  Architecture s = ARMv7_A \<and> 
-                              Extensions s = {} \<and>
-                              PID (FCSEIDR(CP15 s)) = 0 \<and>
-                              PSR.M (CPSR s) \<in> {0x10, 0x1F} \<and>
-                              \<not>HSCTLR.M (HSCTLR(CP15 s))  \<and>
-                              VSCTLR.M (VSCTLR(CP15 s)) \<and>
-                              TTBCR.N (TTBCR(CP15 s)) = 0 \<and> 
-                              \<not>TTBCR.PD0 (TTBCR(CP15 s))  \<and> 
-                              \<not>reg'TTBR0 (TTBR0 (CP15 s)) !! 0 \<and>
-                              \<not>VSCTLR.EE (VSCTLR(CP15 s)) \<and>
-                              \<not>VSCTLR.AFE (VSCTLR(CP15 s)) \<and>  \<comment> \<open>hardware access flag is disabled\<close>
-                              VSCTLR.TRE (VSCTLR(CP15 s))"
+    apply (clarsimp simp: mainTLB_evict_def)
+    apply ((rule wp)+ ; clarsimp?)
+      apply (clarsimp simp: write'unified_mainTLB_def)
+      apply ((rule wp)+ ; clarsimp?)
+     apply (clarsimp simp: mainTLBEntries_def)
+    apply (clarsimp simp: for_loop.simps)
+     apply ((rule wp)+; (clarsimp simp: unified_mainTLB_def write'unified_mainTLB_def)?)
+   
+apply clarsimp
+ apply (rule wp)+ apply clarsimp
+apply (rule wp)
+apply (rule wp)
+apply (rule wp)
+apply (rule wp)
+apply (rule wp)
+apply (rule wp)
+apply (rule wp)
+apply (rule wp)
+
+  (*
+  apply (rule wp_pre)
+  apply (clarsimp simp:  TranslateAddress_def )
+  apply (rule wp)+
+  apply (clarsimp simp: mainTLB_evict_def)
+    apply (rule wp)+
+  apply (clarsimp simp: for_loop.simps write'unified_mainTLB_def)
+ apply (rule wp)+
+  apply (clarsimp simp: microInstrTLBEntries_def)
+ apply (clarsimp simp: for_loop.simps unified_mainTLB_def write'unified_mainTLB_def)
+  *)
+ oops
 
 
-
-fun
-  mem_typcast :: "TLB.MemType_t \<Rightarrow> ARM_Monadic.MemType_t"
-where
-  "mem_typcast TLB.MemType_Normal = ARM_Monadic.MemType_Normal"
-| "mem_typcast TLB.MemType_Device = ARM_Monadic.MemType_Device"
-| "mem_typcast TLB.MemType_StronglyOrdered = ARM_Monadic.MemType_StronglyOrdered"
-
-
-definition
-  mematr_typcast :: "TLB.MemoryAttributes \<Rightarrow> ARM_Monadic.MemoryAttributes"
-where
-  "mematr_typcast mematr = \<lparr> 
-     MemType         = mem_typcast (TLB.MemoryAttributes.MemType mematr),
-     innerattrs      = TLB.MemoryAttributes.innerattrs mematr,
-     innerhints      = TLB.MemoryAttributes.innerhints mematr,
-     innertransient  = TLB.MemoryAttributes.innertransient mematr,
-     outerattrs      = TLB.MemoryAttributes.outerattrs mematr,
-     outerhints      = TLB.MemoryAttributes.outerhints mematr,
-     outershareable  = TLB.MemoryAttributes.outershareable mematr,
-     outertransient  = TLB.MemoryAttributes.outertransient mematr,
-     shareable       = TLB.MemoryAttributes.shareable mematr\<rparr>"
-
-
-fun
-  excp_typcast :: "ARM_Monadic.exception \<Rightarrow> MMU_Translate_Refine.Exception"
-where
-  "excp_typcast (ARM_Monadic.ASSERT string)                  = MMU_Translate_Refine.ASSERT string"
-| "excp_typcast (ARM_Monadic.IMPLEMENTATION_DEFINED string)  = MMU_Translate_Refine.IMPLEMENTATION_DEFINED string"
-| "excp_typcast (ARM_Monadic.MMU_Exception string)           = MMU_Translate_Refine.MMU_Exception string"
-| "excp_typcast  ARM_Monadic.NoException                      = MMU_Translate_Refine.NoException "
-| "excp_typcast (ARM_Monadic.UNPREDICTABLE string)           = MMU_Translate_Refine.UNPREDICTABLE string"
-| "excp_typcast (ARM_Monadic.VFP_EXCEPTION string)           = MMU_Translate_Refine.VFP_EXCEPTION string"
-
-
-
-definition
-  state_comp :: "state \<Rightarrow> tlbs_set cstate_scheme \<Rightarrow> bool"
-where
-  "state_comp s t \<equiv>  
-      (\<lambda>p. (MEM s) (addr_val p)) = heap t \<and>
-      (Addr (reg'TTBR0 (TTBR0 (CP15 s) ) ) ) = ttbr0 t \<and> 
-      ASID (CONTEXTIDR (CP15 s) )   = cstate.asid t \<and>
-      excp_typcast(exception  s) = cstate.Exception t \<and>      
-      (reg'PRRR (PRRR (CP15 s) ) )  = prrr t \<and>
-      (reg'NMRR (NMRR (CP15 s) ) )  = nmrr t \<and>
-      (reg'DACR (DACR (CP15 s) ) )  = dacr t"
-
-consts tlbtypcastt :: "TLBEntry \<Rightarrow> tlb_entry"
-
-definition
-  tlb_rel :: "state \<Rightarrow> tlbs_set cstate_scheme \<Rightarrow> bool"
-where
-  "tlb_rel s t \<equiv>  state_comp s t \<and>
-                  tlbtypcastt ` {entry. \<forall>ad. (micro_DataTLB s) ad = Some entry} \<subseteq> dtlb_set (cstate.more t) \<and> 
-                  tlbtypcastt ` {entry. \<forall>ad. (micro_InstrTLB s) ad = Some entry} \<subseteq> itlb_set (cstate.more t) \<and> 
-                  tlbtypcastt ` {entry. \<forall>ad. (main_TLB s) ad = Some entry} \<subseteq> unitlb_set (cstate.more t) "
-
-
- (*
-consistent and exception
-
- *)
 
 (*
-
-definition
-  "consistent0 m asid ttbr0 tlb va \<equiv>
-     lookup tlb asid (addr_val va) = Hit (pt_walk asid m ttbr0 va) \<or>
-     lookup tlb asid (addr_val va) = Miss"
-
-
-abbreviation
-  "consistent (s::tlb_entry set state_scheme) \<equiv>
-               consistent0 (MEM s) (ASID s) (TTBR0 s) (state.more s)"
-
-*)
-
-
-definition 
-  typ_tlb :: "'a tlb_state_scheme \<Rightarrow> tlbs_set cstate_scheme"
-where
-  "typ_tlb s =  cstate.extend (cstate.truncate s) (tlbs_set s)"
-
-
-
-definition 
-  map_mem :: "(32 word \<Rightarrow> 8 word option) \<Rightarrow> (paddr \<Rightarrow> 8 word option)"
-where 
-  "map_mem m = (\<lambda>x. m (addr_val x))"
-
 lemma  
   "\<lbrakk>MMU_config_assert_isa s;  tlb_rel s (typ_tlb t); 
      TranslateAddress (va , ispriv, iswrite, siz, data_exe) s = (adrdesc, s') ; 
      mmu_translate  (Addr va) siz ispriv iswrite data_exe (t :: 'a tlb_state_scheme) = ((pa' , mematr), t')\<rbrakk> \<Longrightarrow>
-         Addr (paddress (adrdesc)) = pa' \<and> 
-         AddressDescriptor.memattrs (adrdesc) = mematr_typcast mematr \<and>  tlb_rel s' (typ_tlb t')"
+         pa' = Addr (paddress (adrdesc)) \<and> 
+         AddressDescriptor.memattrs (adrdesc) = mematr_typcast' mematr \<and>  tlb_rel s' (typ_tlb t')"
+ oops
+
+lemma
+  "valid (\<lambda>s. MMU_config_assert_isa s \<and> tlb_rel s (typ_tlb t)) 
+     TranslateAddress (va , ispriv, iswrite, siz, data_exe)
+     (\<lambda>adrdesc s'. 
+     mmu_translate  (Addr va) siz ispriv iswrite data_exe (t :: 'a tlb_state_scheme) = ((pa' , mematr), t') \<longrightarrow>
+         pa'    = Addr (paddress (adrdesc)) \<and> 
+         mematr = mematr_typcast (AddressDescriptor.memattrs (adrdesc)) \<and> tlb_rel s' (typ_tlb t'))"
+*)
+
+
+  
 
 (* exception function *)
 
@@ -171,119 +191,6 @@ lemma sanity_check_MMU_config_assert:
   by (clarsimp simp: MMU_config_assert_def MMU_config_assert_isa_def  bind_def split_def read_state_def
                    split:if_split_asm)
 
-
-definition 
-  "mmu_config f \<equiv> 
-        (\<forall> s s'. snd (f s) = s' \<longrightarrow>
-                 MMU_config_assert_isa s \<longrightarrow> MMU_config_assert_isa s' )"
-
-
-lemma mmu_config_bind [intro!, simp]:
-  "\<lbrakk> mmu_config f; \<forall> x. mmu_config (g x) \<rbrakk> \<Longrightarrow> mmu_config (bind f g)"
-  apply (clarsimp simp: mmu_config_def bind_def)
-  by (clarsimp simp: split_def)
-
-
-
-lemma mmu_config_if_else [intro!, simp]:
-  "\<lbrakk> b \<longrightarrow> mmu_config f; \<not>b \<longrightarrow> mmu_config g \<rbrakk> \<Longrightarrow> 
-     mmu_config (\<lambda>s. if b then f s else g s ) "
-  by (clarsimp simp: mmu_config_def split: if_split_asm)
-
-lemma mmu_config_if_else' [intro!, simp]:
-  "\<lbrakk> b \<longrightarrow> mmu_config f; \<not>b \<longrightarrow> mmu_config g \<rbrakk> \<Longrightarrow> 
-     mmu_config (if b then f else g ) "
-  by (clarsimp simp: mmu_config_def split: if_split_asm)
-
-lemma mmu_config_pair_simp [intro!, simp]:
-  "mmu_config (Pair ())"
-  by (clarsimp simp: mmu_config_def)
-  
-
-lemma mmu_config_read_st_simp [intro!, simp]:
-  "mmu_config (read_state f)"
-  by (clarsimp simp: mmu_config_def)
-
-
-lemma mmu_config_update_st_mem_simp [intro!, simp]:
-  "mmu_config (update_state (MEM_update v))"
-  by (clarsimp simp: mmu_config_def MMU_config_assert_isa_def bind_def read_state_def)
-
-
-lemma mmu_config_raise_excp [intro!, simp]:
-  "mmu_config (raise'exception e)"
-  apply (clarsimp simp: mmu_config_def raise'exception_def fst_def snd_def)
-  by (clarsimp simp: bind_def read_state_def update_state_def MMU_config_assert_isa_def split: if_split_asm)
-
-
-lemma mmu_config_pair_simp' [intro!, simp]:
-  "mmu_config (Pair p)"
-  by (clarsimp simp: mmu_config_def)
-
-lemma mmu_config_pair_raise_excp' [intro!, simp]:
-  "mmu_config (case x of None \<Rightarrow> raise'exception (UNPREDICTABLE ''undefined memory'') | Some v \<Rightarrow> Pair v)"
-  by (clarsimp split: option.splits)
-
-
-lemma mmu_config_pair_mem1 [intro!, simp]:
-  "mmu_config (mem1 p)"
-  apply (clarsimp simp: mem1_def)
-  apply (rule mmu_config_bind; clarsimp)
-  by (rule mmu_config_bind; clarsimp simp:  option.splits) 
-  
-
-
-lemma mmu_config_pair_mem [intro!, simp]:
-  "mmu_config (mem (p, n))"
-  by (clarsimp simp: mem_def)
- 
-
-lemma mmu_config_pair_write_mem [intro!, simp]:
-  "mmu_config (write'mem (bl, p, n))"
-  by (clarsimp simp: write'mem_def)
-
-
-lemma mmu_config_translation_root [intro!, simp]:
-  "mmu_config (translation_root va)"
-  by (clarsimp simp: translation_root_def)
-
-
-lemma mmu_config_HaveSecurityExt [intro!, simp]:
-  "mmu_config (HaveSecurityExt ())"
-  by (clarsimp simp: HaveSecurityExt_def)
-
-lemma mmu_config_level1_desc_address_and_desc:
-  "mmu_config (level1_desc_address_and_desc (a, b, mva))"
-  sorry
-
-lemma mmu_config_level2_desc_address_and_desc:
-  "mmu_config (level2_desc_address_and_desc (b, mva, a))"
-  sorry
-
-
-lemma mmu_config_writing_access_flag:
-  "mmu_config (writing_access_flag (a, b, c, d, e ,f, g ,h, i, j,k, l, m))"
-  by (clarsimp simp: writing_access_flag_def)
-
-lemma mmu_config_TLBResult:
-  "mmu_config (TLBResult (a, b, c, d, e, f, g, h, i, j, k, l))"
-  apply (clarsimp simp: TLBResult_def)
-  sorry
-
-
-lemma word_mask_two_bits_false [simp]:
-  "\<lbrakk>n < 31; ucast ((w:: 32 word) && 3) \<noteq> (0 :: 2 word); ucast (w && 3) \<noteq> (1 :: 2 word); 
-      ucast (w && 3) \<noteq> (2 :: 2 word); ucast (w && 3) \<noteq> (3 :: 2 word)\<rbrakk> \<Longrightarrow> False"
-   apply word_bitwise
-  by force
-
-lemma remaining_induct_n[simp]:
-  "\<lbrakk>word_extract (Suc n) n (w:: 32 word) \<noteq> (0 :: 2 word);
-    word_extract (Suc n) n w \<noteq> (1 :: 2 word);
-    word_extract (Suc n) n w \<noteq> (2 :: 2 word);
-    word_extract (Suc n) n w \<noteq> (3 :: 2 word); (n:: nat) < 32 ;  n < 31 \<rbrakk> \<Longrightarrow> False"
-  apply (clarsimp simp: word_extract_def word_bits_def mask_def )
-  by (frule_tac w = "(w >> n)" in  word_mask_two_bits_false; clarsimp)
 
 
 lemma mmu_config_TranslationTableWalkSD:
